src/cbor/CBOR.Spec.Type.fsti
@@ -21,6 +21,8 @@ module U8 = FStar.UInt8
 module U64 = FStar.UInt64
 module FS = FStar.FiniteSet.Base
 module FSA = FStar.FiniteSet.Ambient
+module R = CBOR.Spec.Raw.Valid
+module U = CBOR.Spec.Util
 
 (* The generic data model *)
 
@@ -131,3 +133,46 @@ val unpack_pack: (c: cbor_case) -> Lemma
 val pack_unpack: (c: cbor) -> Lemma
   (ensures (pack (unpack c) == c))
   [SMTPat (unpack c)]
+
+val mk_cbor (r: R.raw_data_item) : Tot cbor
+
+val mk_cbor_equiv (r1 r2: R.raw_data_item) : Lemma
+  (requires (
+    R.valid_raw_data_item r1 == true /\
+    R.valid_raw_data_item r2 == true
+  ))
+  (ensures (
+    R.raw_equiv r1 r2 <==> mk_cbor r1 == mk_cbor r2
+  ))
+
+let mk_cbor_match_map_elem
+  (r: list (R.raw_data_item & R.raw_data_item))
+  (m: cbor_map)
+  (x: R.raw_data_item)
+: Tot prop
+= R.valid_raw_data_item x ==>
+  begin match U.list_setoid_assoc R.raw_equiv x r, cbor_map_get m (mk_cbor x) with
+  | None, None -> True
+  | Some v1, Some v2 -> R.valid_raw_data_item v1 /\ mk_cbor v1 == v2
+  | _ -> False
+  end
+
+let mk_cbor_match_map
+  (r: list (R.raw_data_item & R.raw_data_item))
+  (m: cbor_map)
+: Tot prop
+= forall (x: R.raw_data_item) . mk_cbor_match_map_elem r m x
+
+val mk_cbor_eq
+  (r: R.raw_data_item)
+: Lemma
+  (requires (R.valid_raw_data_item r == true))
+  (ensures (match r, unpack (mk_cbor r) with
+  | R.Simple v1, CSimple v2 -> v1 == v2
+  | R.Int64 ty1 v1, CInt64 ty2 v2 -> ty1 == ty2 /\ v1.value == v2
+  | R.String ty1 _ v1, CString ty2 v2 -> ty1 == ty2 /\ v1 == v2
+  | R.Tagged tag1 v1, CTagged tag2 v2 -> tag1.value == tag2 /\ mk_cbor v1 == v2
+  | R.Map _ v1, CMap v2 -> mk_cbor_match_map v1 v2
+  | R.Array _ v1, CArray v2 -> List.Tot.map mk_cbor v1 == v2
+  | _ -> False
+  ))
